Define CoreChaseTree and prove universality

ExistentialRules/ChaseSequence/CoreChase/Universality.lean
@@ -5,188 +5,144 @@ Released under Apache 2.0 license as described in the file LICENSE.
 
 module
 
+public import ExistentialRules.ChaseSequence.Deterministic
+import ExistentialRules.ChaseSequence.Universality
+
 import ExistentialRules.ChaseSequence.CoreChase.Basic
 public import ExistentialRules.ChaseSequence.CoreChase.CoreChaseBranch
+public import ExistentialRules.ChaseSequence.CoreChase.CoreChaseTree
 
 /-!
 # Universality of the Core Chase Result
 
-Just as for determistic `RegularChaseBranch`es, the result of a determistic `CoreChaseBranch` is a universal model of the underlying `KnowledgeBase`.
+Just as for `RegularChaseTree`s, the result of a `CoreChaseTree` is a universal model set of the underlying `KnowledgeBase`.
+Also, for determistic `CoreChaseBranch`es, result is a universal model.
 -/
 
+public section
+
 variable {sig : Signature} [DecidableEq sig.P] [DecidableEq sig.C] [DecidableEq sig.V]
+
+section CoreChaseTreeUniversality
+
+namespace CoreChaseTree
+
+variable {kb : KnowledgeBase sig}
+
+open AuxiliaryDefsAndTheoremsForUniversalityProof
+
+theorem universal_result (ct : CoreChaseTree kb) (terminates : ct.terminates) : ∀ (m : FactSet sig), m.modelsKb kb ->
+    ∃ (fs : FactSet sig) (h : GroundTermMapping sig), fs ∈ CoreTreeDerivation.result ct.toTreeDerivation terminates ∧ h.isHomomorphism fs m := by
+
+  have trg_inactive_of_fresh_term_present : ∀ (node : ct.NodeWithAddress) (trg : RTrigger (RestrictedObsolescence sig) kb.rules) i lt t, t ∈ trg.val.fresh_terms_for_head_disjunct i lt -> t ∈ (CoreChaseNode.coreChaseNodeInstance.outgoingFacts node.node).terms -> ¬ trg.val.active (CoreChaseNode.coreChaseNodeInstance.outgoingFacts node.node) := by
+    intro node trg i lt t t_fresh t_mem_node trg_act
+    rw [node.node.outgoingFacts_eq] at t_mem_node
+    rw [node.node.outgoingFacts_eq] at trg_act
+    rcases ct.trigger_introducing_functional_term_occurs_in_chase node (FactSet.terms_subset_of_subset node.node.homSubset.left _ t_mem_node) t_fresh
+      with ⟨node2, node2_prec, orig, orig_mem, orig_equiv, head_idx_eq⟩
+    exact ct.origin_trg_remains_inactive node2_prec _ orig_mem _ orig_equiv trg_act
+
+  intro m m_is_model
+
+  let derivs_with_homs := infinite_list_of_derivations_and_homomorphisms CoreChaseNode.out_sub_in ct m m_is_model trg_inactive_of_fresh_term_present
+  let deriv := (head_infinite_list_of_derivations_and_homomorphisms CoreChaseNode.out_sub_in ct m m_is_model trg_inactive_of_fresh_term_present).fst
+  let branch := ct.chaseBranch_for_branch (branch := deriv) mem_branches_fst_head_infinite_list_of_derivations_and_homomorphisms
+
+  let target_idx := (deriv.branch.toList_of_finite (terminates _ mem_branches_fst_head_infinite_list_of_derivations_and_homomorphisms)).length - 1
+  suffices (derivs_with_homs.get? target_idx).map (fun step => step.fst.head.core) = some (CoreChaseDerivation.result branch.toChaseDerivation (terminates _ mem_branches_fst_head_infinite_list_of_derivations_and_homomorphisms)) by
+    have isSome : (derivs_with_homs.get? target_idx).isSome := by
+      rw [Option.map_eq_some_iff] at this; rcases this with ⟨_, eq, _⟩; simp [eq]
+    let step := (derivs_with_homs.get? target_idx).get isSome
+    have step_eq_result : step.fst.head.core = CoreChaseDerivation.result branch.toChaseDerivation (terminates _ mem_branches_fst_head_infinite_list_of_derivations_and_homomorphisms) := by
+      rw [← Option.some_get isSome, Option.map_some, Option.some_inj] at this; exact this
+    exists CoreChaseDerivation.result branch.toChaseDerivation (terminates _ mem_branches_fst_head_infinite_list_of_derivations_and_homomorphisms)
+    exists step.snd
+    constructor
+    . exists deriv, mem_branches_fst_head_infinite_list_of_derivations_and_homomorphisms
+    . rw [← step_eq_result]
+      apply each_step_isHomomorphism_in_infinite_list_of_derivations_and_homomorphisms
+      rw [derivs_with_homs.mem_iff]
+      exists target_idx
+      simp [step]
+  simp only [CoreChaseDerivation.result, ChaseDerivationSkeleton.last]
+  rw [List.getLast_eq_getElem, ← Option.map_some, ← List.getElem?_eq_getElem]
+  rw [PossiblyInfiniteList.getElem?_toList_of_finite]
+  simp only [branch, ChaseTree.chaseBranch_for_branch]
+  simp only [deriv, fst_head_infinite_list_of_derivations_and_homomorphisms_eq_list_of_all_heads]
+  rw [PossiblyInfiniteList.get?_map, Option.map_map]
+  congr
+  simp only [← fst_head_infinite_list_of_derivations_and_homomorphisms_eq_list_of_all_heads]; rfl
+
+end CoreChaseTree
+
+end CoreChaseTreeUniversality
+
+
+section CoreChaseDeterministic
+
+namespace CoreTreeDerivation
+
+variable {rules : RuleSet sig}
+
+/-- The `firstResult` is the result of the `firstBranch`. -/
+def firstResult (td : CoreTreeDerivation rules) (terminates : td.terminates) : FactSet sig := CoreChaseDerivation.result td.firstBranch (terminates _ td.firstBranch_mem_branches)
+
+/-- The `firstResult` is a member of the `TreeDerivation.result`. -/
+theorem firstResult_mem_result {td : CoreTreeDerivation rules} {terminates : td.terminates} : td.firstResult terminates ∈ td.result terminates := by
+  unfold CoreTreeDerivation.result
+  exists td.firstBranch; constructor
+  . rfl
+  . exact td.firstBranch_mem_branches
+
+end CoreTreeDerivation
+
+namespace CoreChaseTree
+
+variable {kb : KnowledgeBase sig}
+
+/-- In the deterministic setting, the `firstResult` of a `CoreChaseTree` is by itself a universal model. -/
+theorem deterministicChaseTreeResultUniversallyModelsKb {ct : CoreChaseTree kb} (det : kb.isDeterministic) (terminates : ct.terminates) :
+    (CoreTreeDerivation.firstResult ct.toTreeDerivation terminates).universallyModelsKb kb := by
+  constructor
+  . apply ct.result_models_kb; exact CoreTreeDerivation.firstResult_mem_result
+  . intro m m_is_model
+    rcases ct.universal_result terminates m m_is_model with ⟨res, hom, res_mem, hom_is_hom⟩
+    unfold CoreTreeDerivation.result at res_mem
+    rcases res_mem with ⟨b, b_mem, res_mem⟩
+    have b_mem := TreeDerivation.branches_eq_firstBranch_of_determinsitic det _ b_mem
+    unfold CoreTreeDerivation.firstResult
+    unfold CoreChaseDerivation.result
+    simp only [← b_mem, res_mem]
+    exact ⟨_, hom_is_hom⟩
+
+end CoreChaseTree
+
+namespace CoreChaseDerivation
+
+variable {rules : RuleSet sig}
+
+/-- The `firstResult` of `intoTree` is the original `ChaseDerivationSkeleton.result`. -/
+theorem firstResult_intoTree_eq_result (cd : CoreChaseDerivation rules) (det : rules.isDeterministic) (terminates : cd.terminates) :
+    CoreTreeDerivation.firstResult (cd.intoTree det) (by unfold TreeDerivation.terminates; intro branch branch_mem; rw [cd.branches_intoTree det _ branch_mem]; exact terminates) = cd.result terminates := by
+  unfold CoreTreeDerivation.firstResult
+  congr
+  exact cd.firstBranch_intoTree_eq_self det
+
+end CoreChaseDerivation
 
 namespace CoreChaseBranch
 
 variable {kb : KnowledgeBase sig}
 
--- TODO: This duplicates a lot of the universality proof of the regular chase derivations. A lot is already generalized over there but it all works on trees, which is why we cannot simply reuse it here... Unify this in the future!
-
-theorem extend_hom_to_next
-    {cb : CoreChaseBranch kb} {cd : CoreChaseDerivation kb.rules} {m : FactSet sig} {h : GroundTermMapping sig} :
-    cd <:+ cb.toChaseDerivation -> kb.isDeterministic -> m.modelsRules kb.rules -> h.isHomomorphism cd.head.core m ->
-    ∀ next ∈ cd.next, ∃ (h' : GroundTermMapping sig), h'.isHomomorphism next.core m := by
-  intro suf det m_is_model h_hom next next_mem
-
-  let orig := next.origin.get (cd.isSome_origin_next next_mem)
-  let trg := orig.fst
-  have trg_act : trg.val.active cd.head.core := cd.active_trigger_origin_next next_mem
-  have trg_rule_det : trg.val.rule.head.length = 1 := by
-    have := det _ trg.property; unfold Rule.isDeterministic at this; rw [decide_eq_true_iff] at this; exact this
-  have orig_snd_zero : orig.snd.val = 0 := by
-    have isLt := orig.snd.isLt; unfold trg at trg_rule_det; simp only [PreTrigger.length_mapped_head, trg_rule_det] at isLt; grind
-
-  let trg_variant_for_m : RTrigger (RestrictedObsolescence sig) kb.rules := {
-    val := {
-      rule := trg.val.rule
-      subs := fun t => h (trg.val.subs t)
-    }
-    property := trg.property
-  }
-  have trg_variant_loaded_for_m : trg_variant_for_m.val.loaded m := by
-    suffices trg_variant_for_m.val.loaded (h.applyFactSet cd.head.core) by
-      exact Set.subset_trans this h_hom.right
-    apply PreTrigger.term_mapping_preserves_loadedness
-    . exact h_hom.left
-    . exact trg_act.left
-  have trg_variant_satisfied_on_m : trg_variant_for_m.val.satisfied_for_disj m ⟨0, by rw [trg_rule_det]; simp⟩ := by
-    suffices trg_variant_for_m.val.satisfied m by
-      rcases this with ⟨idx, goal⟩
-      have : idx = ⟨0, by rw [trg_rule_det]; simp⟩ := by have isLt := idx.isLt; simp only [trg_variant_for_m, trg_rule_det] at isLt; grind
-      simp only [this] at goal
-      exact goal
-    have m_models_rule : m.modelsRule trg_variant_for_m.val.rule := by exact m_is_model trg.val.rule trg.property
-    unfold FactSet.modelsRule at m_models_rule
-    apply m_models_rule
-    apply trg_variant_loaded_for_m
-
-  rcases trg_variant_satisfied_on_m with ⟨obs_for_m_subs, obs_for_m_subs_spec⟩
-
-  let next_hom : GroundTermMapping sig := fun t =>
-    let t_in_node := t ∈ cd.head.core.terms
-    have t_in_node_dec := Classical.propDecidable t_in_node
-    if t_in_node then h t else
-      let t_fresh := t ∈ trg.val.fresh_terms_for_head_disjunct 0 (by rw [trg_rule_det]; simp)
-      have t_fresh_dec := Classical.propDecidable t_fresh
-      if t_fresh_true : t_fresh then
-        obs_for_m_subs (trg.val.existential_var_for_fresh_term _ _ t t_fresh_true)
-      else t
-
-  have next_hom_id_const : next_hom.isIdOnConstants := by
-    intro c
-    simp only [next_hom]
-    split
-    . exact h_hom.left
-    . split
-      case isFalse _ => rfl
-      case isTrue h => rcases trg.val.term_functional_of_mem_fresh_terms _ h with ⟨_, _, _, contra⟩; have contra := Eq.symm contra; simp [GroundTerm.func_neq_const] at contra
-
-  exists next_hom; constructor; exact next_hom_id_const
-  intro mapped_f
-  rw [GroundTermMapping.mem_applyFactSet]
-  intro ⟨f, f_mem, mapped_f_eq⟩
-  have f_mem := next.homSubset.left _ f_mem
-  rw [← CoreChaseNode.ingoingFacts_eq, cd.facts_next next_mem] at f_mem
-  rw [mapped_f_eq]
-  cases f_mem with
-  | inl f_mem =>
-    apply h_hom.right
-    rw [GroundTermMapping.mem_applyFactSet]
-    exists f; rw [CoreChaseNode.outgoingFacts_eq] at f_mem; simp only [f_mem, true_and]
-    apply TermMapping.apply_generalized_atom_congr_left
-    intro t t_mem
-    have t_mem : t ∈ cd.head.core.terms := by exists f
-    simp [next_hom, t_mem]
-  | inr f_mem =>
-    have f_mem : f ∈ trg.val.mapped_head[0] := by
-      rw [List.mem_toSet, ChaseNode.origin_result_eq _ (trg := trg.val.toPreTrigger) (i := 0)] at f_mem; exact f_mem
-      . rfl
-      . exact Eq.symm orig_snd_zero
-    apply obs_for_m_subs_spec.right
-    rw [List.mem_toSet]
-    rw [GroundSubstitution.apply_function_free_conj, TermMapping.apply_generalized_atom_list]
-    rw [List.mem_map]
-    exists (trg.val.atom_for_result_fact ⟨0, by rw [PreTrigger.length_mapped_head, trg_rule_det]; simp⟩ f_mem); constructor
-    . apply PreTrigger.atom_for_result_fact_mem_head
-    conv => right; rw [← trg.val.apply_on_atom_for_result_fact_is_fact ⟨0, by rw [PreTrigger.length_mapped_head, trg_rule_det]; simp⟩ f_mem]
-    rw [← PreTrigger.apply_subs_for_atom_eq]
-    unfold GroundTermMapping.applyFact
-    rw [← Function.comp_apply (f := TermMapping.apply_generalized_atom next_hom)]
-    rw [← GroundTermMapping.applyFact.eq_def, ← GroundSubstitution.apply_function_free_atom_compose_of_isIdOnConstants _ _ next_hom_id_const]
-    apply TermMapping.apply_generalized_atom_congr_left
-    intro voc voc_mem
-    cases voc with
-    | const c => simp [GroundSubstitution.apply_var_or_const]
-    | var v =>
-      rw [GroundSubstitution.apply_var_or_const_compose_of_isIdOnConstants _ _ next_hom_id_const]
-      rw [Function.comp_apply, PreTrigger.apply_subs_for_var_or_const_eq]
-      simp only [GroundSubstitution.apply_var_or_const]
-      cases Decidable.em (v ∈ trg.val.rule.frontier) with
-      | inl v_front =>
-        rw [obs_for_m_subs_spec.left v v_front]
-        rw [PreTrigger.apply_to_var_or_const_frontier_var _ _ _ v_front]
-        simp only [trg_variant_for_m, next_hom]
-        suffices trg.val.subs v ∈ cd.head.core.terms by simp [this]
-        apply FactSet.terms_subset_of_subset trg_act.left
-        rw [FactSet.mem_terms_toSet, PreTrigger.mem_terms_mapped_body_iff]
-        apply Or.inr
-        exists v; constructor
-        . apply Rule.frontier_subset_vars_body; exact v_front
-        . rfl
-      | inr v_front =>
-        have v_exis : v ∈ trg.val.rule.existential_vars_for_head_disjunct 0 (by rw [trg_rule_det]; simp) := by
-          simp only [Rule.existential_vars_for_head_disjunct, List.mem_filter, decide_eq_true_eq]; constructor
-          . rw [FunctionFreeConjunction.mem_vars];
-            exists (trg.val.atom_for_result_fact ⟨0, by rw [PreTrigger.length_mapped_head, trg_rule_det]; simp⟩ f_mem); constructor
-            . apply PreTrigger.atom_for_result_fact_mem_head
-            . exact voc_mem
-          . exact v_front
-        have func_term_fresh : trg.val.functional_term_for_var 0 v ∈ trg.val.fresh_terms_for_head_disjunct 0 (by rw [trg_rule_det]; simp) := by apply List.mem_map_of_mem; exact v_exis
-        rw [PreTrigger.apply_to_var_or_const_non_frontier_var _ _ _ v_front]
-        simp only [next_hom]
-        suffices ¬ trg.val.functional_term_for_var 0 v ∈ cd.head.core.terms by
-          simp only [this, ↓reduceIte]
-          simp only [func_term_fresh, ↓reduceDIte]
-          rw [PreTrigger.existential_var_for_fresh_term_after_functional_term_for_var]
-          exact v_exis
-        intro contra
-        -- from here this is a bit different than for the regular chase derivation
-        rcases cb.trigger_introducing_functional_term_occurs_in_chase ⟨cd.head, cd.mem_of_mem_suffix suf _ cd.head_mem⟩ (FactSet.terms_subset_of_subset cd.head.homSubset.left _ contra) func_term_fresh with ⟨node2, prec, orig2, orig2_mem, equiv, orig2_snd_zero⟩
-        apply cb.origin_trg_remains_inactive prec _ orig2_mem _ equiv
-        exact trg_act
-
-theorem extend_hom_to_each
-    {cb : CoreChaseBranch kb} {cd : CoreChaseDerivation kb.rules} {m : FactSet sig} {h : GroundTermMapping sig} :
-    cd <:+ cb.toChaseDerivation -> kb.isDeterministic -> m.modelsRules kb.rules -> h.isHomomorphism cd.head.core m ->
-    ∀ node ∈ cd, ∃ (h' : GroundTermMapping sig), h'.isHomomorphism node.core m := by
-  intro suf det m_is_model h_hom node node_mem
-  let node : cd.Node := ⟨node, node_mem⟩
-  show ∃ (h' : GroundTermMapping sig), h'.isHomomorphism node.val.core m
-  induction node using cd.mem_rec with
-  | head => exists h
-  | step cd2 suf2 ih next next_mem =>
-    rcases ih with ⟨ig_h, ih_h_hom⟩
-    exact cb.extend_hom_to_next (PossiblyInfiniteList.IsSuffix_trans suf2 suf) det m_is_model ih_h_hom next next_mem
-
-theorem extend_hom_prec
-    {cb : CoreChaseBranch kb} {m : FactSet sig} {h : GroundTermMapping sig} :
-    kb.isDeterministic -> m.modelsRules kb.rules ->
-    ∀ (n1 n2 : cb.Node), n1 ≼ n2 -> h.isHomomorphism n1.val.core m -> ∃ (h' : GroundTermMapping sig), h'.isHomomorphism n2.val.core m := by
-  intro det m_is_model n1 n2 prec h_hom
-  rw [cb.predecessor_iff] at prec; rcases prec with ⟨cd, suf, head_eq, n2_mem⟩
-  exact extend_hom_to_each suf det m_is_model (by rw [head_eq]; exact h_hom) _ n2_mem
-
-public theorem result_universallyModels_kb {cb : CoreChaseBranch kb} (det : kb.isDeterministic) (term : cb.terminates) :
-    (CoreChaseDerivation.result cb.toChaseDerivation term).universallyModelsKb kb := by
-  constructor; exact cb.result_models_kb term
-  intro m m_is_model
-  suffices GroundTermMapping.isHomomorphism id cb.head.core m by
-    exact cb.extend_hom_prec det m_is_model.right ⟨cb.head, cb.head_mem⟩ ⟨cb.last term, cb.last_mem term⟩ (cb.each_prec_last term _) this
-  apply GroundTermMapping.isHomomorphism_id_of_subset
-  intro f f_mem
-  apply m_is_model.left
-  rw [← cb.database_first'.right.left, CoreChaseNode.outgoingFacts_eq]
-  exact f_mem
+theorem result_universallyModels_kb {cb : CoreChaseBranch kb} (det : kb.isDeterministic) (terminates : cb.terminates) :
+    (CoreChaseDerivation.result cb.toChaseDerivation terminates).universallyModelsKb kb := by
+  unfold CoreChaseDerivation.result
+  have eq := CoreChaseDerivation.firstResult_intoTree_eq_result cb.toChaseDerivation det terminates
+  unfold CoreChaseDerivation.result at eq
+  rw [← eq]
+  apply CoreChaseTree.deterministicChaseTreeResultUniversallyModelsKb (ct := (cb.intoTree det)) det
 
 end CoreChaseBranch
+
+end CoreChaseDeterministic
 
